moving some modules from Platform.* to FStar.*

ulib/FStar.Tcp.fst
@@ -1,23 +1,47 @@
-module FStar.Tcp
-open FStar.Bytes
-open FStar.All
+module Platform.Tcp
 
-assume new type stream
-assume new type listener
+open FStar.HyperHeap
 
+open Platform.Bytes
+open Platform.Error
+
+assume new type networkStream: Type0
+assume new type tcpListener: Type0
+
+assume HasEq_networkStream: hasEq networkStream
+
+assume val set_nonblock: networkStream -> unit
+assume val clear_nonblock: networkStream -> unit
 
 (* Server side *)
 
-assume val listen: host:string -> port:int -> ML listener
-assume val accept: l:listener -> ML stream
-assume val stop: l:listener -> ML unit
+assume val listen: string -> nat -> EXT tcpListener
+assume val acceptTimeout: nat -> tcpListener -> EXT networkStream
+assume val accept: tcpListener -> EXT networkStream
+assume val stop: tcpListener -> EXT unit
 
 (* Client side *)
 
-assume val connect: host:string -> port:int -> ML stream
+assume val connectTimeout: nat -> string -> nat -> EXT networkStream
+assume val connect: string -> nat -> EXT networkStream
 
 (* Input/Output *)
 
-assume val read: s:stream -> n:int -> ML (option bytes)
-assume val write: s:stream -> b:bytes -> ML (option unit)
-assume val close: s:stream -> ML unit
+// adding support for (potentially) non-blocking I/O
+// NB for now, send *fails* on partial writes, and *loops* on EAGAIN/EWOULDBLOCK.
+
+type recv_result (max:nat) = 
+  | RecvWouldBlock
+  | RecvError of string
+  | Received of b:bytes {length b <= max}
+assume val recv_async: networkStream -> max:nat -> EXT (recv_result max)
+
+assume val recv: networkStream -> max:nat -> EXT (optResult string (b:bytes {length b <= max}))
+assume val send: networkStream -> bytes -> EXT (optResult string unit)
+assume val close: networkStream -> EXT unit
+
+(* Create a network stream from a given stream.
+   Only used by the application interface TLSharp. *)
+(* assume val create: System.IO.Stream -> NetworkStream*)
+
+ 
